libraries/theories/Type/Nat.v
@@ -406,7 +406,16 @@ Definition sub@{i | } : Nat@{i} -> Nat@{i} -> Prod@{i i} Nat@{i} Nat@{i} :=
 
 (* from: originally defined by Hexirp *)
 Definition div@{i | }
-  : DSum Nat@{i} (fun x => IsTrue (lt zero x)) ->
-    Nat@{i} -> Prod@{i i} Nat@{i} Nat@{i}.
+  : Refinement@{i} Nat@{i} (lt zero) -> Nat@{i} -> Prod@{i i} Nat@{i} Nat@{i}.
 Proof.
+  refine (fun xr y => _).
+  refine (match xr with make_Refinement _ _ x xHT => _ end).
+  refine (match xHT with make_IsTrue xH => _ end).
+  refine (let t0 := _ in t0 xH).
+  refine (match x with zero => _ | succ xp => _ end).
+  -
+    admit.
+  -
+    refine (fun xH' => _).
+    admit.
 Admitted.
